\begin{lemma}[equivalence respects pullback]\label[lemma]{equivalence respects pullback}
Let $\cat{C}$ be a category.
Let $a,b,c \in \cat{C}$.
Let $f: b\rightarrow a$ and $g: c \rightarrow a$.
Let $p: g \rightarrow f \in \overcat{C}{a}$.
Then $Q^g \spull{u(p)}= \spull{p} Q^f$
\end{lemma}

\begin{proof}
Let $R\in \sievecat{f}$.
Let $h \in \spull{p}R^f(t)$ for some $t\in \overcat{C}{a}$. 
Then $ph \in R^f(t)$, so $ph \in R(\dom{t})$ and $t = fph$.
This implies $h\in \spull{p}R(\dom{t})$ and since $g = fp$ also that $t = gh$.
Hence $h\in (\spull{u(p)}R)_g(t)$.

Let $h \in (\spull{u(p)}R)_g(t)$ for some $t\in \overcat{C}{a}$.
Then $h \in \spull{u(p)}R(\dom{t})$ and $t = gh$.
So we get $ph \in R(\dom{t})$ and $t = fph$, 
so $ph\in R^f(t)$.
Hence also $h\in \spull{p}R^f(t)$.
\end{proof}
