\begin{definition}[Relative topology]
Let $\site{C}{T}$ be a site.
Let $a \in \cat{C}$.

The topology $\top{T}$ induces a topology $\top{T}_a$
on $\overcat{C}{a}$ as follows.
Let $f : b \rightarrow a \in \overcat{C}{a}$.
Let $R \in \top{T}{b}$.
Define the sieve $R_f \subset \y{f}$ as follows.
Let $g : b' \rightarrow a \in \overcat{C}{a}$
\[ R_f(g) = \set{p: b' \rightarrow b \in R(b') \suchthat g = f \circ p}.
\]

This is a sieve because if $p\in R_f(g)$ 
and $h : g' \rightarrow g$ arbitrary, 
then $gh=fph$ so $ph \in R_f(gh)$.

Set $\top{T}_a(f) = \set{ R_f \with R \in \top{T}{b}}$.

\end{definition}

\begin{remark}
Every sieve $S$ on $f: b \rightarrow a$ can be considered as a sieve $S'$
on $b$ by defining $S'(b') = \bigcup_g S(g)$ 
with $g: b' \rightarrow b$.
This is clearly a sieve.
We have $S'_f = S$ and $(S_f)' = S$.
Hence $S\in \top{T}{b}$ \iff $S_f\in \top{T}_a(b)$.
\end{remark}

\begin{lemma}
$\top{T}_a$ defines a Grothendieck topology
\end{lemma}

\begin{proof}
We will prove the axioms one by one.

- Axiom 1

Let $p: b' \rightarrow b \in \y{f}(g)$ with $g: b' \rightarrow a$.
Then $g = f \circ p$ hence $p \in \maxsieve{b}_f(g)$
so $\maxsieve{b}_f = \y{f} = \maxsieve{f}$. 
This proves that $\maxsieve{f} \in \top{T}_a(f)$.

- Axiom 2

Let $p: b' \rightarrow b \in \y{f}{g}$ with $g: b' \rightarrow a$.
Let $R_f \in \top{T}_a(f)$.
We have to show that $p^*R_f \in \top{T}_a(g)$.
We will prove $p^*R_f = (p^*R)_g$, which implies the desired result.

Let $h \in p^*R_f(t)$ for some $t\in \overcat{C}{a}$. 
Then $ph \in R_f(t)$, so $ph \in R(\dom{t})$ and $t = fph$.
This implies $h\in p^*R(\dom{t})$ and since $g = fp$ also that $t = gh$.
Hence $h\in (p^*R)_g(t)$.

Let $h \in (p^*R)_g(t)$ for some $t\in \overcat{C}{a}$.
Then $h \in p^*R(\dom{t})$ and $t = gh$.
So we get $ph \in R(\dom{t})$ and $t = fph$, 
so $ph\in R_f(t)$.
Hence also $h\in p^*R_f(t)$.

- Axiom 3

Let $R_f \in \top{T}_a(f)$.
Let $S_f$ be any sieve on $f$ for some sieve $S$ on $b$.
Any sieve on $f$ can be written as $S_f$ for some $S$ by the above remark %TODO: ref
Assume that $p^*S_f \in \top{T}_a(g)$ 
for any $p: b' \rightarrow b \in R_f(g)$
with $g: b' \rightarrow a$.

By assumption $p^*S_f = (p^*S)_g$ is covering for any $p \in R_f(g)$,
hence $p^*S$ is covering for any $p \in R(b')$, 
hence $S$ is covering so $S_f$ is.
\end{proof}